Final Translatable Spec

asset/tmp/impl/rsl/Message.i.dfy
@@ -1,1 +1,118 @@
-Error: TopLevel.find_module: not found: (Internal.NonEmptyList.:: ("LiveRSL__Message_i", []))
+include ""
+
+
+module Impl_LiveRSL__Message_i 
+{
+
+	datatype CMessage = 
+	CMessage_Invalid(
+		
+	)
+	 | 
+	CMessage_Request(
+		seqno_req: int, 
+		val: CAppMessage
+	)
+	 | 
+	CMessage_1a(
+		bal_1a: CBallot
+	)
+	 | 
+	CMessage_1b(
+		bal_1b: CBallot, 
+		log_truncation_point: COperationNumber, 
+		votes: CVotes
+	)
+	 | 
+	CMessage_2a(
+		bal_2a: CBallot, 
+		opn_2a: COperationNumber, 
+		val_2a: CRequestBatch
+	)
+	 | 
+	CMessage_2b(
+		bal_2b: CBallot, 
+		opn_2b: COperationNumber, 
+		val_2b: CRequestBatch
+	)
+	 | 
+	CMessage_Heartbeat(
+		bal_heartbeat: CBallot, 
+		suspicious: bool, 
+		opn_ckpt: COperationNumber
+	)
+	 | 
+	CMessage_Reply(
+		seqno_reply: int, 
+		reply: CAppMessage
+	)
+	 | 
+	CMessage_AppStateRequest(
+		bal_state_req: CBallot, 
+		opn_state_req: COperationNumber
+	)
+	 | 
+	CMessage_AppStateSupply(
+		bal_state_supply: CBallot, 
+		opn_state_supply: COperationNumber, 
+		app_state: CAppState, 
+		reply_cache: CReplyCache
+	)
+	 | 
+	CMessage_StartingPhase2(
+		bal_2: CBallot, 
+		logTruncationPoint_2: COperationNumber
+	)
+
+	predicate CMessageIsValid(s: CMessage) 
+	{
+		match s
+		case CMessage_Invalid() => CMessageIsAbstractable(s)
+		case CMessage_Request(seqno_req, val) => CMessageIsAbstractable(s) && CAppMessageIsValid(s.val)
+		case CMessage_1a(bal_1a) => CMessageIsAbstractable(s) && CBallotIsValid(s.bal_1a)
+		case CMessage_1b(bal_1b, log_truncation_point, votes) => CMessageIsAbstractable(s) && CBallotIsValid(s.bal_1b) && COperationNumberIsValid(s.log_truncation_point) && CVotesIsValid(s.votes)
+		case CMessage_2a(bal_2a, opn_2a, val_2a) => CMessageIsAbstractable(s) && CBallotIsValid(s.bal_2a) && COperationNumberIsValid(s.opn_2a) && CRequestBatchIsValid(s.val_2a)
+		case CMessage_2b(bal_2b, opn_2b, val_2b) => CMessageIsAbstractable(s) && CBallotIsValid(s.bal_2b) && COperationNumberIsValid(s.opn_2b) && CRequestBatchIsValid(s.val_2b)
+		case CMessage_Heartbeat(bal_heartbeat, suspicious, opn_ckpt) => CMessageIsAbstractable(s) && CBallotIsValid(s.bal_heartbeat) && COperationNumberIsValid(s.opn_ckpt)
+		case CMessage_Reply(seqno_reply, reply) => CMessageIsAbstractable(s) && CAppMessageIsValid(s.reply)
+		case CMessage_AppStateRequest(bal_state_req, opn_state_req) => CMessageIsAbstractable(s) && CBallotIsValid(s.bal_state_req) && COperationNumberIsValid(s.opn_state_req)
+		case CMessage_AppStateSupply(bal_state_supply, opn_state_supply, app_state, reply_cache) => CMessageIsAbstractable(s) && CBallotIsValid(s.bal_state_supply) && COperationNumberIsValid(s.opn_state_supply) && CAppStateIsValid(s.app_state) && CReplyCacheIsValid(s.reply_cache)
+		case CMessage_StartingPhase2(bal_2, logTruncationPoint_2) => CMessageIsAbstractable(s) && CBallotIsValid(s.bal_2) && COperationNumberIsValid(s.logTruncationPoint_2)
+
+	}
+
+	predicate CMessageIsAbstractable(s: CMessage) 
+	{
+		match s
+		case CMessage_Invalid() => true
+		case CMessage_Request(seqno_req, val) => CAppMessageIsAbstractable(s.val)
+		case CMessage_1a(bal_1a) => CBallotIsAbstractable(s.bal_1a)
+		case CMessage_1b(bal_1b, log_truncation_point, votes) => CBallotIsAbstractable(s.bal_1b) && COperationNumberIsAbstractable(s.log_truncation_point) && CVotesIsAbstractable(s.votes)
+		case CMessage_2a(bal_2a, opn_2a, val_2a) => CBallotIsAbstractable(s.bal_2a) && COperationNumberIsAbstractable(s.opn_2a) && CRequestBatchIsAbstractable(s.val_2a)
+		case CMessage_2b(bal_2b, opn_2b, val_2b) => CBallotIsAbstractable(s.bal_2b) && COperationNumberIsAbstractable(s.opn_2b) && CRequestBatchIsAbstractable(s.val_2b)
+		case CMessage_Heartbeat(bal_heartbeat, suspicious, opn_ckpt) => CBallotIsAbstractable(s.bal_heartbeat) && COperationNumberIsAbstractable(s.opn_ckpt)
+		case CMessage_Reply(seqno_reply, reply) => CAppMessageIsAbstractable(s.reply)
+		case CMessage_AppStateRequest(bal_state_req, opn_state_req) => CBallotIsAbstractable(s.bal_state_req) && COperationNumberIsAbstractable(s.opn_state_req)
+		case CMessage_AppStateSupply(bal_state_supply, opn_state_supply, app_state, reply_cache) => CBallotIsAbstractable(s.bal_state_supply) && COperationNumberIsAbstractable(s.opn_state_supply) && CAppStateIsAbstractable(s.app_state) && CReplyCacheIsAbstractable(s.reply_cache)
+		case CMessage_StartingPhase2(bal_2, logTruncationPoint_2) => CBallotIsAbstractable(s.bal_2) && COperationNumberIsAbstractable(s.logTruncationPoint_2)
+
+	}
+
+	function AbstractifyCMessageToRslMessage(s: CMessage) : RslMessage 
+		requires CMessageIsAbstractable(s)
+	{
+		match s
+		case CMessage_Invalid() => RslMessage_Invalid()
+		case CMessage_Request(seqno_req, val) => RslMessage_Request(s.seqno_req, AbstractifyCAppMessageToAppMessage(s.val))
+		case CMessage_1a(bal_1a) => RslMessage_1a(AbstractifyCBallotToBallot(s.bal_1a))
+		case CMessage_1b(bal_1b, log_truncation_point, votes) => RslMessage_1b(AbstractifyCBallotToBallot(s.bal_1b), AbstractifyCOperationNumberToOperationNumber(s.log_truncation_point), AbstractifyCVotesToVotes(s.votes))
+		case CMessage_2a(bal_2a, opn_2a, val_2a) => RslMessage_2a(AbstractifyCBallotToBallot(s.bal_2a), AbstractifyCOperationNumberToOperationNumber(s.opn_2a), AbstractifyCRequestBatchToRequestBatch(s.val_2a))
+		case CMessage_2b(bal_2b, opn_2b, val_2b) => RslMessage_2b(AbstractifyCBallotToBallot(s.bal_2b), AbstractifyCOperationNumberToOperationNumber(s.opn_2b), AbstractifyCRequestBatchToRequestBatch(s.val_2b))
+		case CMessage_Heartbeat(bal_heartbeat, suspicious, opn_ckpt) => RslMessage_Heartbeat(AbstractifyCBallotToBallot(s.bal_heartbeat), s.suspicious, AbstractifyCOperationNumberToOperationNumber(s.opn_ckpt))
+		case CMessage_Reply(seqno_reply, reply) => RslMessage_Reply(s.seqno_reply, AbstractifyCAppMessageToAppMessage(s.reply))
+		case CMessage_AppStateRequest(bal_state_req, opn_state_req) => RslMessage_AppStateRequest(AbstractifyCBallotToBallot(s.bal_state_req), AbstractifyCOperationNumberToOperationNumber(s.opn_state_req))
+		case CMessage_AppStateSupply(bal_state_supply, opn_state_supply, app_state, reply_cache) => RslMessage_AppStateSupply(AbstractifyCBallotToBallot(s.bal_state_supply), AbstractifyCOperationNumberToOperationNumber(s.opn_state_supply), AbstractifyCAppStateToAppState(s.app_state), AbstractifyCReplyCacheToReplyCache(s.reply_cache))
+		case CMessage_StartingPhase2(bal_2, logTruncationPoint_2) => RslMessage_StartingPhase2(AbstractifyCBallotToBallot(s.bal_2), AbstractifyCOperationNumberToOperationNumber(s.logTruncationPoint_2))
+
+	}
+}
