asset/tmp/impl/rsl/Types.i.dfy
@@ -1,1 +1,251 @@
-Error: TopLevel.find_module: not found: (Internal.NonEmptyList.:: ("LiveRSL__Types_i", []))
+include ""
+
+
+module Impl_LiveRSL__Types_i 
+{
+	type COperationNumber = int
+
+	predicate COperationNumberIsAbstractable(s: COperationNumber) 
+	{
+		true
+	}
+
+	predicate COperationNumberIsValid(s: COperationNumber) 
+	{
+		COperationNumberIsAbstractable(s)
+	}
+
+	function AbstractifyCOperationNumberToOperationNumber(s: COperationNumber) : OperationNumber 
+		requires COperationNumberIsAbstractable(s)
+	{
+		s
+	}
+
+	datatype CBallot = 
+	CBallot(
+		seqno: int, 
+		proposer_id: int
+	)
+
+	predicate CBallotIsValid(s: CBallot) 
+	{
+		CBallotIsAbstractable(s)
+	}
+
+	predicate CBallotIsAbstractable(s: CBallot) 
+	{
+		true
+	}
+
+	function AbstractifyCBallotToBallot(s: CBallot) : Ballot 
+		requires CBallotIsAbstractable(s)
+	{
+		Ballot(s.seqno, s.proposer_id)
+	}
+
+	datatype CRequest = 
+	CRequest(
+		client: EndPoint, 
+		seqno: int, 
+		request: CAppMessage
+	)
+
+	predicate CRequestIsValid(s: CRequest) 
+	{
+		CRequestIsAbstractable(s) 
+		&& 
+		EndPointIsValid(s.client) 
+		&& 
+		CAppMessageIsValid(s.request)
+	}
+
+	predicate CRequestIsAbstractable(s: CRequest) 
+	{
+		EndPointIsAbstractable(s.client) 
+		&& 
+		CAppMessageIsAbstractable(s.request)
+	}
+
+	function AbstractifyCRequestToRequest(s: CRequest) : Request 
+		requires CRequestIsAbstractable(s)
+	{
+		Request(AbstractifyEndPointToNodeIdentity(s.client), s.seqno, AbstractifyCAppMessageToAppMessage(s.request))
+	}
+
+	datatype CReply = 
+	CReply(
+		client: EndPoint, 
+		seqno: int, 
+		reply: CAppMessage
+	)
+
+	predicate CReplyIsValid(s: CReply) 
+	{
+		CReplyIsAbstractable(s) 
+		&& 
+		EndPointIsValid(s.client) 
+		&& 
+		CAppMessageIsValid(s.reply)
+	}
+
+	predicate CReplyIsAbstractable(s: CReply) 
+	{
+		EndPointIsAbstractable(s.client) 
+		&& 
+		CAppMessageIsAbstractable(s.reply)
+	}
+
+	function AbstractifyCReplyToReply(s: CReply) : Reply 
+		requires CReplyIsAbstractable(s)
+	{
+		Reply(AbstractifyEndPointToNodeIdentity(s.client), s.seqno, AbstractifyCAppMessageToAppMessage(s.reply))
+	}
+	type CRequestBatch = seq<CRequest>
+
+	predicate CRequestBatchIsAbstractable(s: CRequestBatch) 
+	{
+		(forall i :: i in s ==> CRequestIsAbstractable(i))
+	}
+
+	predicate CRequestBatchIsValid(s: CRequestBatch) 
+	{
+		CRequestBatchIsAbstractable(s) 
+		&& 
+		(forall i :: i in s ==> CRequestIsValid(i))
+	}
+
+	function AbstractifyCRequestBatchToRequestBatch(s: CRequestBatch) : RequestBatch 
+		requires CRequestBatchIsAbstractable(s)
+	{
+		AbstractifySeq(s, AbstractifyCRequestToRequest)
+	}
+	type CReplyCache = map<EndPoint, CReply>
+
+	predicate CReplyCacheIsAbstractable(s: CReplyCache) 
+	{
+		(forall i :: i in s ==> EndPointIsAbstractable(i) && CReplyIsAbstractable(s[i]))
+	}
+
+	predicate CReplyCacheIsValid(s: CReplyCache) 
+	{
+		CReplyCacheIsAbstractable(s) 
+		&& 
+		(forall i :: i in s ==> EndPointIsValid(i) && CReplyIsValid(s[i]))
+	}
+
+	function AbstractifyCReplyCacheToReplyCache(s: CReplyCache) : ReplyCache 
+		requires CReplyCacheIsAbstractable(s)
+	{
+		AbstractifyMap(s, AbstractifyEndPointToNodeIdentity, AbstractifyReplyToCReply, AbstractifyNodeIdentityToEndPoint)
+	}
+
+	datatype CVote = 
+	CVote(
+		max_value_bal: CBallot, 
+		max_val: CRequestBatch
+	)
+
+	predicate CVoteIsValid(s: CVote) 
+	{
+		CVoteIsAbstractable(s) 
+		&& 
+		CBallotIsValid(s.max_value_bal) 
+		&& 
+		CRequestBatchIsValid(s.max_val)
+	}
+
+	predicate CVoteIsAbstractable(s: CVote) 
+	{
+		CBallotIsAbstractable(s.max_value_bal) 
+		&& 
+		CRequestBatchIsAbstractable(s.max_val)
+	}
+
+	function AbstractifyCVoteToVote(s: CVote) : Vote 
+		requires CVoteIsAbstractable(s)
+	{
+		Vote(AbstractifyCBallotToBallot(s.max_value_bal), AbstractifyCRequestBatchToRequestBatch(s.max_val))
+	}
+	type CVotes = map<COperationNumber, CVote>
+
+	predicate CVotesIsAbstractable(s: CVotes) 
+	{
+		(forall i :: i in s ==> COperationNumberIsAbstractable(i) && CVoteIsAbstractable(s[i]))
+	}
+
+	predicate CVotesIsValid(s: CVotes) 
+	{
+		CVotesIsAbstractable(s) 
+		&& 
+		(forall i :: i in s ==> COperationNumberIsValid(i) && CVoteIsValid(s[i]))
+	}
+
+	function AbstractifyCVotesToVotes(s: CVotes) : Votes 
+		requires CVotesIsAbstractable(s)
+	{
+		AbstractifyMap(s, AbstractifyCOperationNumberToOperationNumber, AbstractifyVoteToCVote, AbstractifyOperationNumberToCOperationNumber)
+	}
+
+	datatype CearnerTuple = 
+	CearnerTuple(
+		received_2b_message_senders: set<EndPoint>, 
+		candidate_learned_value: CRequestBatch
+	)
+
+	predicate CearnerTupleIsValid(s: CearnerTuple) 
+	{
+		CearnerTupleIsAbstractable(s) 
+		&& 
+		(forall i :: i in s.received_2b_message_senders ==> EndPointIsValid(i)) 
+		&& 
+		CRequestBatchIsValid(s.candidate_learned_value)
+	}
+
+	predicate CearnerTupleIsAbstractable(s: CearnerTuple) 
+	{
+		(forall i :: i in s.received_2b_message_senders ==> EndPointIsAbstractable(i)) 
+		&& 
+		CRequestBatchIsAbstractable(s.candidate_learned_value)
+	}
+
+	function AbstractifyCearnerTupleToLearnerTuple(s: CearnerTuple) : LearnerTuple 
+		requires CearnerTupleIsAbstractable(s)
+	{
+		LearnerTuple(AbstractifySet(s.received_2b_message_senders, AbstractifyEndPointToNodeIdentity), AbstractifyCRequestBatchToRequestBatch(s.candidate_learned_value))
+	}
+	type CearnerState = map<COperationNumber, CearnerTuple>
+
+	predicate CearnerStateIsAbstractable(s: CearnerState) 
+	{
+		(forall i :: i in s ==> COperationNumberIsAbstractable(i) && CearnerTupleIsAbstractable(s[i]))
+	}
+
+	predicate CearnerStateIsValid(s: CearnerState) 
+	{
+		CearnerStateIsAbstractable(s) 
+		&& 
+		(forall i :: i in s ==> COperationNumberIsValid(i) && CearnerTupleIsValid(s[i]))
+	}
+
+	function AbstractifyCearnerStateToLearnerState(s: CearnerState) : LearnerState 
+		requires CearnerStateIsAbstractable(s)
+	{
+		AbstractifyMap(s, AbstractifyCOperationNumberToOperationNumber, AbstractifyLearnerTupleToCearnerTuple, AbstractifyOperationNumberToCOperationNumber)
+	}
+
+	function method CBalLt(ba: CBallot, bb: CBallot) : bool 
+		requires CBallotIsValid(ba)
+		requires CBallotIsValid(bb)
+		ensures var lr := BalLt(AbstractifyCBallotToBallot(ba), AbstractifyCBallotToBallot(bb)); var cr := CBalLt(ba, bb); (cr) == (lr)
+	{
+		(ba.seqno < bb.seqno) || (ba.seqno == bb.seqno && ba.proposer_id < bb.proposer_id)
+	}
+
+	function method CBalLeq(ba: CBallot, bb: CBallot) : bool 
+		requires CBallotIsValid(ba)
+		requires CBallotIsValid(bb)
+		ensures var lr := BalLeq(AbstractifyCBallotToBallot(ba), AbstractifyCBallotToBallot(bb)); var cr := CBalLeq(ba, bb); (cr) == (lr)
+	{
+		(ba.seqno < bb.seqno) || (ba.seqno == bb.seqno && ba.proposer_id <= bb.proposer_id)
+	}
+}
