asset/tmp/impl/kv/Configuration.i.dfy
@@ -1,0 +1,62 @@
+include ""
+
+
+module Impl_SHT__Configuration_i 
+{
+
+	datatype CSHTConfiguration = 
+	CSHTConfiguration(
+		clientIds: seq<EndPoint>, 
+		hostIds: seq<EndPoint>, 
+		rootIdentity: EndPoint, 
+		params: CParameters
+	)
+
+	predicate CSHTConfigurationIsValid(s: CSHTConfiguration) 
+	{
+		CSHTConfigurationIsAbstractable(s) 
+		&& 
+		(forall i :: i in s.clientIds ==> EndPointIsValid(i)) 
+		&& 
+		(forall i :: i in s.hostIds ==> EndPointIsValid(i)) 
+		&& 
+		EndPointIsValid(s.rootIdentity) 
+		&& 
+		CParametersIsValid(s.params)
+	}
+
+	predicate CSHTConfigurationIsAbstractable(s: CSHTConfiguration) 
+	{
+		(forall i :: i in s.clientIds ==> EndPointIsAbstractable(i)) 
+		&& 
+		(forall i :: i in s.hostIds ==> EndPointIsAbstractable(i)) 
+		&& 
+		EndPointIsAbstractable(s.rootIdentity) 
+		&& 
+		CParametersIsAbstractable(s.params)
+	}
+
+	function AbstractifyCSHTConfigurationToSHTConfiguration(s: CSHTConfiguration) : SHTConfiguration 
+		requires CSHTConfigurationIsAbstractable(s)
+	{
+		SHTConfiguration(AbstractifySeq(s.clientIds, AbstractifyEndPointToNodeIdentity), AbstractifySeq(s.hostIds, AbstractifyEndPointToNodeIdentity), AbstractifyEndPointToNodeIdentity(s.rootIdentity), AbstractifyCParametersToParameters(s.params))
+	}
+
+	function method CHostsDistinct(hostIds: seq<EndPoint>, i: int, j: int) : bool 
+		requires (forall i :: i in hostIds ==> EndPointIsValid(i))
+		ensures CHostsDistinct(hostIds, i, j) == HostsDistinct(AbstractifySeq(hostIds, AbstractifyEndPointToNodeIdentity), i, j)
+	{
+		0 <= i && i < |hostIds| && 0 <= j && j < |hostIds| && hostIds[i] == hostIds[j] ==> i == j
+	}
+
+	function method CWFSHTConfiguration(c: CSHTConfiguration) : bool 
+		requires CSHTConfigurationIsValid(c)
+		ensures CWFSHTConfiguration(c) == WFSHTConfiguration(AbstractifyCSHTConfigurationToSHTConfiguration(c))
+	{
+		0 < |c.hostIds| 
+		&& 
+		c.rootIdentity in c.hostIds 
+		&& 
+		(forall i, j :: CHostsDistinct(c.hostIds, i, j))
+	}
+}
