asset/tmp/impl/kv/Message.i.dfy
@@ -1,0 +1,73 @@
+include ""
+
+
+module Impl_SHT__Message_i 
+{
+
+	datatype CMessage = 
+	CGetRequest(
+		k_getrequest: Key
+	)
+	 | 
+	CSetRequest(
+		k_setrequest: Key, 
+		v_setrequest: COptionalValue
+	)
+	 | 
+	CReply(
+		k_reply: Key, 
+		v: COptionalValue
+	)
+	 | 
+	CRedirect(
+		k_redirect: Key, 
+		id: EndPoint
+	)
+	 | 
+	CShard(
+		kr: KeyRange, 
+		recipient: EndPoint
+	)
+	 | 
+	CDelegate(
+		range: KeyRange, 
+		h: Hashtable
+	)
+
+	predicate CMessageIsValid(s: CMessage) 
+	{
+		match s
+		case CGetRequest(k_getrequest) => CMessageIsAbstractable(s) && KeyIsValid(s.k_getrequest)
+		case CSetRequest(k_setrequest, v_setrequest) => CMessageIsAbstractable(s) && KeyIsValid(s.k_setrequest) && COptionalValueIsValid(s.v_setrequest)
+		case CReply(k_reply, v) => CMessageIsAbstractable(s) && KeyIsValid(s.k_reply) && COptionalValueIsValid(s.v)
+		case CRedirect(k_redirect, id) => CMessageIsAbstractable(s) && KeyIsValid(s.k_redirect) && EndPointIsValid(s.id)
+		case CShard(kr, recipient) => CMessageIsAbstractable(s) && KeyRangeIsValid(s.kr) && EndPointIsValid(s.recipient)
+		case CDelegate(range, h) => CMessageIsAbstractable(s) && KeyRangeIsValid(s.range) && HashtableIsValid(s.h)
+
+	}
+
+	predicate CMessageIsAbstractable(s: CMessage) 
+	{
+		match s
+		case CGetRequest(k_getrequest) => KeyIsAbstractable(s.k_getrequest)
+		case CSetRequest(k_setrequest, v_setrequest) => KeyIsAbstractable(s.k_setrequest) && COptionalValueIsAbstractable(s.v_setrequest)
+		case CReply(k_reply, v) => KeyIsAbstractable(s.k_reply) && COptionalValueIsAbstractable(s.v)
+		case CRedirect(k_redirect, id) => KeyIsAbstractable(s.k_redirect) && EndPointIsAbstractable(s.id)
+		case CShard(kr, recipient) => KeyRangeIsAbstractable(s.kr) && EndPointIsAbstractable(s.recipient)
+		case CDelegate(range, h) => KeyRangeIsAbstractable(s.range) && HashtableIsAbstractable(s.h)
+
+	}
+
+	function AbstractifyCMessageToMessage(s: CMessage) : Message 
+		requires CMessageIsAbstractable(s)
+	{
+		match s
+		case CGetRequest(k_getrequest) => GetRequest(AbstractifyKeyToKey(s.k_getrequest))
+		case CSetRequest(k_setrequest, v_setrequest) => SetRequest(AbstractifyKeyToKey(s.k_setrequest), AbstractifyCOptionalValueToOptionalValue(s.v_setrequest))
+		case CReply(k_reply, v) => Reply(AbstractifyKeyToKey(s.k_reply), AbstractifyCOptionalValueToOptionalValue(s.v))
+		case CRedirect(k_redirect, id) => Redirect(AbstractifyKeyToKey(s.k_redirect), AbstractifyEndPointToNodeIdentity(s.id))
+		case CShard(kr, recipient) => Shard(AbstractifyKeyRangeToKeyRange(s.kr), AbstractifyEndPointToNodeIdentity(s.recipient))
+		case CDelegate(range, h) => Delegate(AbstractifyKeyRangeToKeyRange(s.range), AbstractifyHashtableToHashtable(s.h))
+
+	}
+}
