asset/tmp/impl/kv/Network.i.dfy
@@ -1,0 +1,103 @@
+include ""
+
+
+module Impl_SHT__Network_i 
+{
+	type CPMsg = CSingleMessage
+
+	predicate CPMsgIsAbstractable(s: CPMsg) 
+	{
+		CSingleMessageIsAbstractable(s)
+	}
+
+	predicate CPMsgIsValid(s: CPMsg) 
+	{
+		CPMsgIsAbstractable(s) 
+		&& 
+		CSingleMessageIsValid(s)
+	}
+
+	function AbstractifyCPMsgToPMsg(s: CPMsg) : PMsg 
+		requires CPMsgIsAbstractable(s)
+	{
+		AbstractifyCSingleMessageToSingleMessage(s)
+	}
+
+	datatype CPacket = 
+	CPacket(
+		dst: EndPoint, 
+		src: EndPoint, 
+		msg: CPMsg
+	)
+
+	predicate CPacketIsValid(s: CPacket) 
+	{
+		CPacketIsAbstractable(s) 
+		&& 
+		EndPointIsValid(s.dst) 
+		&& 
+		EndPointIsValid(s.src) 
+		&& 
+		CPMsgIsValid(s.msg)
+	}
+
+	predicate CPacketIsAbstractable(s: CPacket) 
+	{
+		EndPointIsAbstractable(s.dst) 
+		&& 
+		EndPointIsAbstractable(s.src) 
+		&& 
+		CPMsgIsAbstractable(s.msg)
+	}
+
+	function AbstractifyCPacketToPacket(s: CPacket) : Packet 
+		requires CPacketIsAbstractable(s)
+	{
+		Packet(AbstractifyEndPointToNodeIdentity(s.dst), AbstractifyEndPointToNodeIdentity(s.src), AbstractifyCPMsgToPMsg(s.msg))
+	}
+	type CNetwork = set<CPacket>
+
+	predicate CNetworkIsAbstractable(s: CNetwork) 
+	{
+		(forall i :: i in s ==> CPacketIsAbstractable(i))
+	}
+
+	predicate CNetworkIsValid(s: CNetwork) 
+	{
+		CNetworkIsAbstractable(s) 
+		&& 
+		(forall i :: i in s ==> CPacketIsValid(i))
+	}
+
+	function AbstractifyCNetworkToNetwork(s: CNetwork) : Network 
+		requires CNetworkIsAbstractable(s)
+	{
+		AbstractifySet(s, AbstractifyCPacketToPacket)
+	}
+
+	function method CNetwork_Init() : CNetwork 
+		ensures var n := CNetwork_Init(); CNetworkIsValid(n) && Network_Init(AbstractifyCNetworkToNetwork(n))
+	{
+		var t1 := 
+			{}; 		
+		t1
+	}
+
+	function method CPacketsTo(ps: set<CPacket>, dst: EndPoint) : set<CPacket> 
+		requires (forall i :: i in ps ==> CPacketIsValid(i))
+		requires EndPointIsValid(dst)
+		ensures var lr := PacketsTo(AbstractifySet(ps, AbstractifyCPacketToPacket), AbstractifyEndPointToNodeIdentity(dst)); var cr := CPacketsTo(ps, dst); (forall i :: i in cr ==> CPacketIsValid(i)) && (AbstractifySet(cr, AbstractifyCPacketToPacket)) == (lr)
+	{
+		[Printer for ... hasn't been implemented.]
+	}
+
+	function method CNetwork_Receive(n: CNetwork, dst: EndPoint) : set<CPacket> 
+		requires CNetworkIsValid(n)
+		requires EndPointIsValid(dst)
+		ensures var recv := CNetwork_Receive(n, dst); (forall i :: i in recv ==> CPacketIsValid(i)) && Network_Receive(AbstractifyCNetworkToNetwork(n), AbstractifyEndPointToNodeIdentity(dst), AbstractifySet(recv, AbstractifyCPacketToPacket))
+	{
+		var t1 := 
+			CPacketsTo(n, dst); 		
+		t1
+	}
+}
