asset/tmp/spec/rsl/Acceptor.i.dfy
@@ -25,13 +25,13 @@ module LiveRSL__Acceptor_i {
     log_truncation_point:OperationNumber
   )
 
-  predicate IsLogTruncationPointValid(log_truncation_point:OperationNumber, last_checkpointed_operation:seq<OperationNumber>,
-                                      config:LConfiguration)
-  {
-    IsNthHighestValueInSequence(log_truncation_point,
-                                last_checkpointed_operation,
-                                LMinQuorumSize(config))
-  }
+  // predicate IsLogTruncationPointValid(log_truncation_point:OperationNumber, last_checkpointed_operation:seq<OperationNumber>,
+  //                                     config:LConfiguration)
+  // {
+  //   IsNthHighestValueInSequence(log_truncation_point,
+  //                               last_checkpointed_operation,
+  //                               LMinQuorumSize(config))
+  // }
   
   predicate RemoveVotesBeforeLogTruncationPoint(votes:Votes, votes':Votes, log_truncation_point:OperationNumber)
   {
@@ -56,7 +56,7 @@ module LiveRSL__Acceptor_i {
     && (forall opn :: opn in votes' ==> votes'[opn] == (if opn == new_opn then new_vote else votes[opn]))
     */
 
-    && (forall opn :: opn in votes' <==> opn >= log_truncation_point && (opn in votes || opn == new_opn))
+    && (forall opn :: opn in votes' <==> opn in (votes.Keys + {new_opn}) && opn >= log_truncation_point)
     && (forall opn :: opn in votes' ==> votes'[opn] == (if opn == new_opn then new_vote else votes[opn]))
   }
 
@@ -70,69 +70,69 @@ module LiveRSL__Acceptor_i {
     && a.log_truncation_point == 0
   }
       
-  predicate LAcceptorProcess1a(s:LAcceptor, s':LAcceptor, inp:RslPacket, broadcast_sent_packets:seq<RslPacket>)
-    requires inp.msg.RslMessage_1a?
-  {
-    var m := inp.msg;
-    if inp.src in s.constants.all.config.replica_ids && BalLt(s.max_bal, m.bal_1a) && LReplicaConstantsValid(s.constants) then
-      && broadcast_sent_packets == [ LPacket(inp.src, s.constants.all.config.replica_ids[s.constants.my_index],
-                                             RslMessage_1b(m.bal_1a, s.log_truncation_point, s.votes)) ]
-      && s' == s.(max_bal := m.bal_1a)
-    else
-      s' == s && broadcast_sent_packets == []
-  }
+  // predicate LAcceptorProcess1a(s:LAcceptor, s':LAcceptor, inp:RslPacket, broadcast_sent_packets:seq<RslPacket>)
+  //   requires inp.msg.RslMessage_1a?
+  // {
+  //   var m := inp.msg;
+  //   if inp.src in s.constants.all.config.replica_ids && BalLt(s.max_bal, m.bal_1a) && LReplicaConstantsValid(s.constants) then
+  //     && broadcast_sent_packets == [ LPacket(inp.src, s.constants.all.config.replica_ids[s.constants.my_index],
+  //                                            RslMessage_1b(m.bal_1a, s.log_truncation_point, s.votes)) ]
+  //     && s' == s.(max_bal := m.bal_1a)
+  //   else
+  //     s' == s && broadcast_sent_packets == []
+  // }
 
-  predicate LAcceptorProcess2a(s:LAcceptor, s':LAcceptor, inp:RslPacket, broadcast_sent_packets:seq<RslPacket>)
-    requires inp.msg.RslMessage_2a?
-    requires inp.src in s.constants.all.config.replica_ids
-    requires BalLeq(s.max_bal, inp.msg.bal_2a)
-    requires LeqUpperBound(inp.msg.opn_2a, s.constants.all.params.max_integer_val)
-  {
-    var m := inp.msg;
-    var newLogTruncationPoint := if inp.msg.opn_2a - s.constants.all.params.max_log_length + 1 > s.log_truncation_point then
-                                   inp.msg.opn_2a - s.constants.all.params.max_log_length + 1
-                                 else
-                                   s.log_truncation_point;
-    && LBroadcastToEveryone(s.constants.all.config, s.constants.my_index, RslMessage_2b(m.bal_2a, m.opn_2a, m.val_2a), broadcast_sent_packets)
-    && s'.max_bal == m.bal_2a
-    && s'.log_truncation_point == newLogTruncationPoint
-    && (if s.log_truncation_point <= inp.msg.opn_2a then
-         LAddVoteAndRemoveOldOnes(s.votes, s'.votes, m.opn_2a, Vote(m.bal_2a, m.val_2a), newLogTruncationPoint)
-       else
-         s'.votes == s.votes
-         )
-         // UNCHANGED
-    && s'.constants == s.constants
-    && s'.last_checkpointed_operation == s.last_checkpointed_operation
-  }
+  // predicate LAcceptorProcess2a(s:LAcceptor, s':LAcceptor, inp:RslPacket, broadcast_sent_packets:seq<RslPacket>)
+  //   requires inp.msg.RslMessage_2a?
+  //   requires inp.src in s.constants.all.config.replica_ids
+  //   requires BalLeq(s.max_bal, inp.msg.bal_2a)
+  //   requires LeqUpperBound(inp.msg.opn_2a, s.constants.all.params.max_integer_val)
+  // {
+  //   var m := inp.msg;
+  //   var newLogTruncationPoint := if inp.msg.opn_2a - s.constants.all.params.max_log_length + 1 > s.log_truncation_point then
+  //                                  inp.msg.opn_2a - s.constants.all.params.max_log_length + 1
+  //                                else
+  //                                  s.log_truncation_point;
+  //   && LBroadcastToEveryone(s.constants.all.config, s.constants.my_index, RslMessage_2b(m.bal_2a, m.opn_2a, m.val_2a), broadcast_sent_packets)
+  //   && s'.max_bal == m.bal_2a
+  //   && s'.log_truncation_point == newLogTruncationPoint
+  //   && (if s.log_truncation_point <= inp.msg.opn_2a then
+  //        LAddVoteAndRemoveOldOnes(s.votes, s'.votes, m.opn_2a, Vote(m.bal_2a, m.val_2a), newLogTruncationPoint)
+  //      else
+  //        s'.votes == s.votes
+  //        )
+  //        // UNCHANGED
+  //   && s'.constants == s.constants
+  //   && s'.last_checkpointed_operation == s.last_checkpointed_operation
+  // }
 
-  predicate LAcceptorProcessHeartbeat(s:LAcceptor, s':LAcceptor, inp:RslPacket)
-    requires inp.msg.RslMessage_Heartbeat?
-  {
-    if inp.src in s.constants.all.config.replica_ids then
-      var sender_index := GetReplicaIndex(inp.src, s.constants.all.config);
-      if 0 <= sender_index < |s.last_checkpointed_operation| && inp.msg.opn_ckpt > s.last_checkpointed_operation[sender_index] then
-        //s' == s[last_checkpointed_operation := s.last_checkpointed_operation[inp.src := inp.msg.opn_ckpt]]
-        s'.last_checkpointed_operation == s.last_checkpointed_operation[sender_index := inp.msg.opn_ckpt]
-        // UNCHANGED
-        && s'.constants == s.constants
-        && s'.max_bal == s.max_bal
-        && s'.votes == s.votes
-        && s'.log_truncation_point == s.log_truncation_point
-      else
-        s' == s
-    else
-      s' == s
-  }
+  // predicate LAcceptorProcessHeartbeat(s:LAcceptor, s':LAcceptor, inp:RslPacket)
+  //   requires inp.msg.RslMessage_Heartbeat?
+  // {
+  //   if inp.src in s.constants.all.config.replica_ids then
+  //     var sender_index := GetReplicaIndex(inp.src, s.constants.all.config);
+  //     if 0 <= sender_index < |s.last_checkpointed_operation| && inp.msg.opn_ckpt > s.last_checkpointed_operation[sender_index] then
+  //       //s' == s[last_checkpointed_operation := s.last_checkpointed_operation[inp.src := inp.msg.opn_ckpt]]
+  //       s'.last_checkpointed_operation == s.last_checkpointed_operation[sender_index := inp.msg.opn_ckpt]
+  //       // UNCHANGED
+  //       && s'.constants == s.constants
+  //       && s'.max_bal == s.max_bal
+  //       && s'.votes == s.votes
+  //       && s'.log_truncation_point == s.log_truncation_point
+  //     else
+  //       s' == s
+  //   else
+  //     s' == s
+  // }
 
-  predicate LAcceptorTruncateLog(s:LAcceptor, s':LAcceptor, opn:OperationNumber)
-  {
-    var t := seq(10, idx => 1);
-    if opn <= s.log_truncation_point then
-      s' == s
-    else
-      && RemoveVotesBeforeLogTruncationPoint(s.votes, s'.votes, opn)
-      && s' == s.(log_truncation_point := opn, votes := s'.votes)
-  }
+  // predicate LAcceptorTruncateLog(s:LAcceptor, s':LAcceptor, opn:OperationNumber)
+  // {
+  //   var t := seq(10, idx => 1);
+  //   if opn <= s.log_truncation_point then
+  //     s' == s
+  //   else
+  //     && RemoveVotesBeforeLogTruncationPoint(s.votes, s'.votes, opn)
+  //     && s' == s.(log_truncation_point := opn, votes := s'.votes)
+  // }
   
 }
